---
title: "Quadratic Shortcuts"
subtitle: "a equals 1"
---

This is called the standard form of a quadratic equation.

$$
ax^2 + bx + c = 0
$$
---- 
<br />

You can solve this equation with the quadratic formula:

$$
x = \frac{-b \pm \sqrt{b^2 - 4ac}}{2a} 
$$
<br />

Or by turning it into something that looks like this:

$$
(x + ...)(x + ...) = 0
$$

But how exactly do you turn this: $ax^2 + bx + c = 0$  
<br />
into this:$(x + ...)(x + ...) = 0$ ? 












Here's a thing: $\sqrt{\frac{1}{2}}$



Here's an aligned environment

$$
\begin{aligned}
x &= \frac{-b \pm \sqrt{b^2 - 4ac}}{2a} \\
&= \frac{-2 \pm \sqrt{-2^2 - (4 \times 5 \times 2)}}{2 \times 5} \\
&= 6.324 \text{ and } 4.324
\end{aligned}
$$

asdfas

$$


\end{aligned}
$$










